\documentclass[a4paper,11pt]{article}
\usepackage[utf8]{inputenc}
\input{prelude}
\input{ldef}
\usepackage{eucal}
\usepackage{url}
\usepackage{tikz}
\usepackage{amsfonts,amsmath}
\usepackage{hyperref}
\begin{document}

\title{Verifying Snapping Mechanism - Connecting Ideal and Flopt}
\author{}

\date{}

\maketitle
In order to verify the differential privacy proeprty of
the snapping mechanism \cite{mironov2012significance},
we follow the logic rules designed from
\cite{barthe2016proving} and connecting 
it with the floating point computation semantics.
\section{Syntax}
\[\begin{array}{llll}
\mbox{Programs} & \prog & ::= & 
	%
     \varx = \expr ~|~ \varx \samplel \edistr
	%
	~|~ \prog ; \prog \\

\mbox{Expr.} & \expr & ::= & \rval 
	%
	~|~ \varx  ~|~ \expr \bop \expr
	%
	~|~ \uop (\expr) \\
%
\mbox{Binary Operation} & \bop & ::= & + ~|~ - ~|~ \times ~|~ \div \\
%
\mbox{Unary Operation} & \uop & ::= & \ln ~|~ - ~|~ \round{\cdot} 
	%
	~|~ \clamp_B(\cdot) \\
%
\mbox{Value} & \valv & ::= & \rval ~|~  \fval \\
%
\mbox{Distr.} & \edistr & ::= & \uniform(0, 1) 
%
	~|~ \uniform\{-1, 1\}\\ 
%
\mbox{Error} & \err & ::= & (\rval, \rval) \\
%
\mbox{Env.} & \trsenv & ::= & \cdot ~|~ \trsenv[x \mapsto (\fval, \err)] \\
%
\mbox{Assert.} & \Phi &  & 
\end{array}
\]
where $\rval$ is in domain of real number $\real$, $\rval \in \real$ and $\fval$ is in domain of floating point number $\float$, $\fval \in \float$. Furthermore, the domain of floating point number $\float$ is a subset of $\real$ containing the real number that can be represented in the floating point computation.

\section{
Connecting Coupling Logic
%
with Floating Point Computation
}
%
\begin{defn}
[$(\epsilon, \delta)$ - lifting \cite{barthe2016proving}]
Two sub-distributions $\mu_1 \in \distr(U_1)$, $\mu_2 \in \distr(U_2)$are related by the $(\epsilon, \delta)$ - dilation lifting of $\Psi \subseteq U_1 \times U_2$, written $\mu_1 \Psi^{\#(\epsilon, \delta)} \mu_2$, if there exist two witness sub-distributions $\mu_L \in \distr(U_1 \times U_2)$ and $\mu_R \in \distr(U_1, U_2)$ s.t.:
\begin{enumerate}
	\item $\projl(\mu_L) = \mu_1$ and $\projr(\mu_R) = \mu_2$;
	\item $\supp(\mu_L) \subseteq \Psi$ and $\supp(\mu_R) \subseteq \Psi$; and
	\item $\Delta_{\epsilon}(\mu_L, \mu_R) \leq \delta$.
\end{enumerate}
\end{defn}
%
Fig. \ref{fig:aprhl} presents the main rules from apRHL excluding the while and condition rules which is not defined in out syntax, as well as the sampling rule, which we generalized in extended apRHL.
The rule in Fig. \ref{fig:aprhlplus} represents the lifting proved in soundness theorem. They all extended from the apRHL+ \cite{barthe2016proving}. This generalization allows apRHL to prove differential privacy using the coupling composition principle when the standard composition theorem is insufficient.
%
\begin{figure}[t]
\boxed{\vdash: prog \times prog \times \real \times Assert \times Assert}\\
\boxed{\Phi: Env \times Env \to bool}\\
\boxed{\pi_i: Value \times Value \times Value \to Value, ~~ i = 1, 2, 3}
\begin{mathpar}
\inferrule*[right = FloptUnif]
{
\empty
}
{
	\vdash
	\varx_1 \samplel \uniform(0, 1) 	
	\sim_{\epsilon} 
	\varx_2 \samplel \uniform(0, 1)
	: 
	\top \Rightarrow  
	% (P \Rightarrow   Q)
	e^{-\epsilon} \pi_2(\varx_2) \leq \pi_3 (\varx_1) 
	\land 
	e^{-\epsilon} \pi_2 (\varx_1) \leq \pi_3 (\varx_2)
}
\and
\inferrule*[right = FloptNull]
{
\empty
}
{
	\vdash 
	\varx_1 \samplel \uniform(0, 1) 	
	\sim_{0} 
	\varx_2 \samplel \uniform(0, 1) 
	: \top \Rightarrow 
	\pi_1 (\varx_2) = \pi_1 (\varx_1 )
	\land \pi_2 (\varx_2) = \pi_2 (\varx_1)
	\land \pi_3 (\varx_2) = \pi_3 (\varx_1)
}
\and
\inferrule*[right = FloptNull2]
{
\empty
}
{
	\vdash 
	\varx_1 \samplel \uniform\{-1, 1\} 	
	\sim_{0} 
	\varx_2 \samplel \uniform\{-1, 1\}  
	: \top \Rightarrow 
	\pi_1 (\varx_2) = \pi_1 (\varx_1 )
	\land \pi_2 (\varx_2) = \pi_2 (\varx_1)
	\land \pi_3 (\varx_2) = \pi_3 (\varx_1)
}
\end{mathpar}
\caption{Rules Extended from apRHL+}
\label{fig:aprhlplus}
\end{figure}

\begin{figure}[t]
\begin{mathpar}
\inferrule*[right = Assn]
{
\expr_1 \trsto (\fval_1, \rval_{l1}, \rval_{u1})
\and
\expr_2 \trsto (\fval_2, \rval_{l2}, \rval_{u2})
}
{
	\vdash 
	\varx_1 = \expr_1  
	\sim_{0} 
	\varx_2 = \expr_2  
	: \Phi[(\fval_1, \rval_{l1}, \rval_{u1})/\varx_1]
	[(\fval_2, \rval_{l2}, \rval_{u2})/\varx_2]  \Rightarrow \Phi
}
\and
\inferrule*[right = Assn]
{
\empty
}
{
	\vdash 
	\varx_1 = \expr_1  
	\sim_{0} 
	\varx_2 = \expr_2  
	: \Phi[\expr_1/\varx_1]
	[\expr_2/\varx_2]  \Rightarrow \Phi
}
~~~
\inferrule*[right = Seq]
{
\prog_1 \sim_{\epsilon} \prog_2 : \Phi_1 \Rightarrow \Phi'_1
\\
\prog'_1 \sim_{\epsilon'} \prog'_2 : \Phi'_1 \Rightarrow \Phi_2
}
{
	\vdash 
	\prog_1; \prog'_1  
	\sim_{\epsilon + \epsilon'} 
	\prog_2; \prog'_2
	: \Phi_1  \Rightarrow  \Phi_2
}
\and
\inferrule*[right = Conseq]
{
\prog_1 \sim_{\epsilon} \prog_2 : \Phi'_1 \Rightarrow \Phi'_2
\and
\Phi_1 \Rightarrow \Phi'_1
\and 
\Phi'_2 \Rightarrow \Phi_2
\and 
\epsilon \leq \epsilon'
}
{
\prog_1 \sim_{\epsilon'} \prog_2 : 
\Phi_1 \Rightarrow \Phi_2
}
\end{mathpar}
\caption{Proving Rules from apRHL}
\label{fig:aprhl}
\end{figure}
The judgment $\vdash \prog_1 \sim_{\epsilon, \delta} \prog_2: \Phi_0 \Rightarrow \Phi$ is read as, given two environments $\trsenv_1$ and $\trsenv_2$ satisfying precondition $\Phi_0$, 
then under the semantics definition, 
$(\sem{\prog_1}_{\trsenv_1})$ 
$\sem{\Phi}^{\#(\epsilon, \delta)}$ 
$(\sem{\prog_2}_{\trsenv_2})$.

\newpage
\paragraph{Semantics.}
$\boxed{Env \times Expr. \trsto Value \times Value \times Value }$
%
\[
	\begin{array}{rcl}
	\sem{\expr}_{\trsenv}
	& \in &  
	\big\{(\fval, \rval_{l}, \rval_{u}) ~|~
	\exists ~~  
	\trsenv,  
	\expr \trsto (\fvalv, \rval_{l}, \rval_{u})\big\}
	\end{array}
\]
%
$
\boxed{Env \times \distr. \trsto 
\distr(Value \times Value \times Value )}
$
%
\[
	\begin{array}{rcl}
	\sem{\uniform(0, 1)}_{\trsenv}
	& \in & 
	\big\{
	(\fval, \rval_{l}, \rval_{u}) ~|~
	\fval \leftarrow \uniform(0, 1)^{\diamond}
	\land \rval_{l} = \rval_{u} = \fval
	\big\}\\
	\sem{\uniform\{-1, 1\}}_{\trsenv}
	& \in & 
	\big\{
	(-1, -1, -1), (1, 1, 1) ~|~
	each ~ w.p. ~ 0.5 
	\big\}\\	
	\end{array}
\]
%
$\boxed{Env \times prog \trsto \distr(Env)}$
\[
	\begin{array}{rcl}
% 	\sem{\eskip}_{\trsenv}
% 	& = & 
% 	~\unit{\trsenv}
% 	\\
	%
	\sem{\varx \samplel \edistr}_{\trsenv}
	& = & 
	\elet (\fval, \rval_{l}, \rval_{u}) = \sem{\edistr}_{\trsenv} 
	\ein 
	\unit{\trsenv[\varx \mapsto (\fval, \rval_{l}, \rval_{u})]}
	\\
	%
	\sem{\varx = \expr}_{\trsenv}
	& = &  
	~\unit{\trsenv[\varx \mapsto \sem{\expr}_{\trsenv}]}
	\\
	%
	\sem{\prog_1; \prog_2}_{\trsenv}
	& = &  \elet  \trsenv_1 = 
	\sem{\prog_1}_{\trsenv} \ein
	\sem{\prog_2}_{\trsenv_1} 
	\end{array}
\]
In the semantics, 
$\trsenv, \expr \trsto (\fvalv, err)$ represents given an environment $\trsenv$, the expression $\expr$
is transited to $\fvalv$ with error bound $err = (\rval_{l}, \rval_{u})$ in floating point transition semantics, s.t. $\rval_{l} \leq \fvalv \leq \rval_{u}$. 
$\trsenv, \prog \trsto \trsenv'$ represents given and environment $\trsenv$, the program $\prog$ is transited to a new environment $\trsenv'$.


\clearpage
\begin{thm}[Soundness]
 $\forall \prog^1$, $\prog^2$,  $ \vdash \prog^1	
\sim_{\epsilon, \delta} 
\prog^2 :
\Phi_0 \Rightarrow \Phi $,    $\forall \trsenv^1_0$, $\trsenv^2_0$ 
s.t $\Phi_0$: 
$\trsenv^1_0 ~ \sem{\Phi_0} ~ \trsenv^2_0$,
then
$$ 
(\sem{\prog^1}_{\trsenv^1_0})  
\sem{\Phi}^{\#(\epsilon, \delta)} 
(\sem{\prog^2}_{\trsenv^2_0}) 
$$.
\end{thm}



\begin{proof}
By induction on the transition judgement $\vdash \prog^1	
\sim_{\epsilon, \delta} 
\prog^2 :
\Phi_0 \Rightarrow \Phi $.
\begin{itemize}
\caseL{[\textsc{FloptUnif}]}
	In this case, 
	$\sem{\Phi} = 
	\{((\fval_1, \rval_{1l}, \rval_{1u}), (\fval_2, \rval_{2l}, \rval_{2u})) 
	\in (\float \times \real \times \real) \times (\float \times \real \times \real)
	|
	\expr^{-\epsilon} \rval_{2l} \leq \rval_{1u}
	\land
	\expr^{\epsilon} \rval_{1l} \leq \rval_{2u}
	\}$
	%
	\\
	%
	By the semantics of sampling, we have:\\
	%
	$\sem{\varx^1 \samplel \edistr^1}_{\trsenv^1_0} = \distr(\trsenv^1)$ and 
	%
	$\sem{\varx^2 \samplel \edistr^2}_{\trsenv^2_0} = \distr(\trsenv^2)$. \\
	%
	By the definition of the environment and the soundness of the transition semantics, we have for any $(\fval_1, \rval_{1l}, \rval_{1u}), (\fval_2, \rval_{2l}, \rval_{2u})$ s.t.,
	%
	$\trsenv^1 (\varx^1) = (\fval_1, \rval_{1l}, \rval_{1u})$
	and
	$\trsenv^2 (\varx^2) = (\fval_2, \rval_{2l}, \rval_{2u})$:
	%
	\\
	%
	$ \rval_{1l} \leq \fval_1 \leq \rval_{1u} ~ (1)$ 
	and
	$ \rval_{2l} \leq \fval_2 \leq \rval_{2u} ~ (2)$.
	%
	\\
	%
	Let $\rval_1$ and $\rval_2$ be the real representation of $\fval_1$ and $\fval_2$ in $\real$, by the soundness of ideal judgment, we have:
	$\pi_1 (\distr(\trsenv^1)) ~ \Psi^{\#(\epsilon, 0)} ~ \pi_1 (\distr(\trsenv^2))$, where
	\[
		\Psi = \{(\rval_1, \rval_2) \in \real \times \real
		| 
		\rval_1 e^{-\epsilon} 
		\leq \rval_2
		\leq \rval_1 e^{\epsilon} \}.
	\]
	By $(1)$ and $(2)$, we have:
	$\Psi \implies \Phi$.
	\\
	So it can be proven by implication that 
	$(\distr(\trsenv^1)) ~ \Phi^{\#(\epsilon, 0)} ~ (\distr(\trsenv^2))$, i.e., 
	$$
	\sem{\varx^1 \samplel \edistr^1}_{\trsenv^1_0} 
		~ \sem{\Phi}^{\#(\epsilon, 0)} ~
		\sem{\varx^2 \samplel \edistr^2}_{\trsenv^2_0}
	$$
\caseL{[\textsc{FloptNull}] }
	In this case, 
	$\sem{\Phi} = 
	\{((\fval_1, \rval_{1l}, \rval_{1u}), (\fval_2, \rval_{2l}, \rval_{2u})) 
	\in (\float \times \real \times \real) \times (\float \times \real \times \real)
	|
	\rval_{2l} = \rval_{1l}
	\land
	\rval_{2u} = \rval_{1u}
	\land
	\fval_1 = \fval_2
	\}$
	%
	\\
	%
	By the semantics of sampling, we have:\\
	%
	$\sem{\varx^1 \samplel \edistr^1}_{\trsenv^1_0} = \distr(\trsenv^1)$ and 
	%
	$\sem{\varx^2 \samplel \edistr^2}_{\trsenv^2_0} = \distr(\trsenv^2)$. \\
	%
	By the definition of the environment and the soundness of the transition semantics, we have for any $(\fval_1, \rval_{1l}, \rval_{1u}), (\fval_2, \rval_{2l}, \rval_{2u})$ s.t.,
	%
	$\trsenv^1 (\varx^1) = (\fval_1, \rval_{1l}, \rval_{1u})$
	and
	$\trsenv^2 (\varx^2) = (\fval_2, \rval_{2l}, \rval_{2u})$:
	%
	\\
	%
	$ \rval_{1l} \leq \fval_1 \leq \rval_{1u} ~ (1)$ 
	and
	$ \rval_{2l} \leq \fval_2 \leq \rval_{2u} ~ (2)$.
	%
	\\
	%
	Let $\rval_1$ and $\rval_2$ be the real representation of $\fval_1$ and $\fval_2$ in $\real$, by the soundness of ideal judgment, we have:
	$\pi_1 (\distr(\trsenv^1)) ~ \Psi^{\#(\epsilon, 0)} ~ \pi_1 (\distr(\trsenv^2))$, where
	\[
		\Psi = \{(\rval_1, \rval_2) \in \real \times \real
		| 
		\rval_1 = \rval_2 \}.
	\]
	By $(1)$ and $(2)$, we have:
	$\Psi \implies \Phi$.
	\\
	So it can be proven by implication that 
	$(\distr(\trsenv^1)) ~ \Phi^{\#(\epsilon, 0)} ~ (\distr(\trsenv^2))$, i.e., 
	$$
	\sem{\varx^1 \samplel \edistr^1}_{\trsenv^1_0} 
		~ \sem{\Phi}^{\#(\epsilon, 0)} ~
		\sem{\varx^2 \samplel \edistr^2}_{\trsenv^2_0}
	$$
	% \caseL{[\textsc{Assn}] }
	% \caseL{[\textsc{Seq}] }
	% \caseL{[\textsc{ConSeq}] }
	\end{itemize}
\end{proof}

\newpage
\begin{thm}
\label{corr_axunif}
Let $\mu_1 \in \distr(\real)$, $\mu_2 \in \distr(\real)$ are defined:
\[
	{\mu_1}(x) = \uniform(x)
\]
\[
	{\mu_2}(y) = {\uniform}(y)
\]
where $\uniform$ is uniform distribution over $[0, 1)$ whoes $\pdf.$ is defined as:
\[
	\pdf_{\uniform}(x) = 
	\begin{cases}
	1 & x \in [0, 1)\\
	0       & o.w.
	\end{cases}.
\]
Then, $\mu_1 \Psi^{\#(\epsilon, 0)} \mu_2$, where
\[
	\Psi = \{(x,y) \in \real \times \real | x \cdot e^{-\epsilon} \leq y \leq x \cdot e^{\epsilon} \}
\]
\end{thm}
\begin{proof}[Proof of Theorem \ref{corr_axunif}]

Existing $\mu_L, \mu_R \in \distr(\real \times \real)$:
\[
	{\mu_L}(x, y) = 
	\begin{cases}
	{\uniform}(x) & x \cdot e^{-\epsilon} = y \land x \in [0, 1)\\
	0       & o.w.
	\end{cases}
	\\
	{\mu_R}(x, y) = 
	\begin{cases}
	{\uniform}(y) & x \cdot e^{-\epsilon} = y \land y \in [0, 1)\\
	0       & o.w.
	\end{cases}.
\]


Their $\pdf.$ are defined:
\[
	\pdf_{\mu_L}(x, y) = 
	\begin{cases}
	\pdf_{\uniform}(x) & x \cdot e^{-\epsilon} = y \land x \in [0, 1)\\
	0       & o.w.
	\end{cases}
\]
\[
	\pdf_{\mu_R}(x, y) = 
	\begin{cases}
	\pdf_{\uniform}(y) & x \cdot e^{-\epsilon} = y \land y \in [0, 1)\\
	0       & o.w.
	\end{cases}.
\]
\begin{itemize}
	\item $\supp(\mu_L) \in \Psi \land \supp(\mu_R) \in \Psi$

	\begin{itemize}
		\item $\supp(\mu_L) \subseteq \Psi$ 

		By definition of the $\pdf$ of $\mu_L$, we have: $\pr{(x,y) \samplel \mu_L}{(x,y) \notin \Psi} = 0$.

		Then we can derive $\supp(\mu_L) \in \Psi$

		\item $\supp(\mu_R) \subseteq \Psi$

		By definition of the $\pdf$ of $\mu_R$, we have: $\pr{(x,y) \samplel \mu_R}{(x,y) \notin \Psi} = 0$.

		Then we can derive $\supp(\mu_L) \in \Psi$

	\end{itemize}		


	\item $\projl(\mu_L) = \mu_1 \land \pi_2(\mu_R) = \mu_2$
	
	\begin{itemize}
		\item $\projl(\mu_L) = \mu_1$ 

		% Equivalent to show $\pdf_{\projl(\mu_L)}  = \pdf_{\mu_1}$.

		By definition of the $\projl$ and $\pdf$ of $\mu_L$, we have $\forall x \in \real$:
		\[
			\pdf_{\projl(\mu_L)}(x) = 
			\begin{cases}
			\int_{y}\pdf_{\uniform}(x) & (x,y) \in \Psi \land x \in [0, 1)\\
			0       & o.w.
			\end{cases} 
			= 
			\begin{cases}
			\pdf_{\uniform}(x) & x \in [0, 1)\\
			0       & o.w.
			\end{cases}
			=
			\pdf_{\mu_1}(x)
		\]

		\item $\projl(\mu_R) = \mu_2$ 

		Equivalent to show$\pdf_{\projr(\mu_R)}  = \pdf_{\mu_2}$.

		By definition of the $\projr$ and $\pdf$ of $\mu_R$, we have $\forall y \in \real$:
		\[
			\pdf_{\projr(\mu_R)}(y) = 
			\begin{cases}
			\int_{x}\pdf_{\uniform}(y) & (x,y) \in \Psi \land y \in [0, 1)\\
			0       & o.w.
			\end{cases} 
			= 
			\begin{cases}
			\pdf_{\uniform}(y) & y \in [0, 1)\\
			0       & o.w.
			\end{cases}
			=
			\pdf_{\mu_2}(y)
		\]
	\end{itemize}	

	\item $\Delta_{\epsilon}(\mu_L, \mu_R) \leq 0$

	By definition of $\epsilon-$DP divergence, we have:
	 \[
	 \begin{array}{ll}
	 \Delta_{\epsilon}(\mu_L, \mu_R) 
	 & = \underset{S}{\psup}
	 \Big(
	 \pr{(x,y) \samplel \mu_L}{(x,y) \in S} - e^{\epsilon} \pr{(x,y) \samplel \mu_R}{(x,y) \in S}
	 \Big) \\
	 & =\underset{S}{\psup}
	 \Big(
	 \int_{(x,y) \in S} \pdf_{\mu_L}(x, y) - e^{\epsilon} \int_{(x,y) \in S} \pdf_{\mu_R}(x, y)
	 \Big)	 
	 \end{array}
	 \]
	 \begin{itemize}
	 	\item[{\bf case}] $S \subseteq \{(x, y) | x \in [0, 1) \land x \cdot e^{-\epsilon} = y\}$:\\
		 \[
		 \begin{array}{ll}
		 \Delta_{\epsilon}(\mu_L, \mu_R) 
		 & = 
		 \int_{(x,y) \in S} \pdf_{\uniform}(x) - e^{\epsilon} \int_{(x,y) \in S} \pdf_{\uniform}(y)\\
		 & = 
		 \int_{(x,y) \in S} \pdf_{\uniform}(x) - e^{\epsilon} \int_{(x,y) \in S} \pdf_{\uniform}(x * e^{-\epsilon})\\ 
		 & = 
		 \int_{(x,y) \in S} \pdf_{\uniform}(x) - e^{\epsilon}* e^{-\epsilon} \int_{(x,y) \in S} \pdf_{\uniform}(x )\\
		 & = 0 
		 \end{array}
		 \]
	 	\item[{\bf case}] $S \subseteq \{(x, y) | x \in [1, e^{\epsilon}) \land x \cdot e^{-\epsilon} = y\}$:\\
		 \[
		 \begin{array}{ll}
		 \Delta_{\epsilon}(\mu_L, \mu_R) 
		 & = 
		 0 - e^{\epsilon} \int_{(x,y) \in S} \pdf_{\uniform}(y)\\
		 & <  0 
		 \end{array}
		 \]
	 	\item[{\bf case}] o.w.\\
		 \[
		 \begin{array}{ll}
		 \Delta_{\epsilon}(\mu_L, \mu_R) 
		 & = 0 - 0 =  0 
		 \end{array}
		 \]	 	

	 \end{itemize}

\end{itemize}
\end{proof}


\newpage
\section{Snapping Mechanism}

\begin{defn}
[$\snap(a) : A \to \distr(\real)$]
Given privacy parameter $\epsilon$, the Snapping mechanism $\snap(a)$ is defined as:
\[
	\varu \samplel \uniform(0,1); s \samplel \uniform\{-1, 1\};
	\varx = \clamp_B \big(
	\round{f(a) + \frac{1}{\epsilon} \times s \times \ln (\varu)}_{\Lambda}
	\big)
\]
where $f(a)$ represents a value that the query function $f$ be evaluated over input database $a \in A$, $\epsilon$ is the privacy parameter, $B$ is the clamping argument and $\Lambda$ is the rounding argument satisfying $\lambda = 2^k$ where $2^k$ is the smallest power of 2 greater or equal to the $\frac{1}{\epsilon}$.
\end{defn}

\begin{thm}[The $\snap$ mechanism is 
$\epsilon-$differentially private]
\end{thm}
\begin{proof}
\tiny{
\begin{mathpar}
\inferrule*[right = Seq]
{
	\inferrule*[right = Seq]
	{
	\inferrule[FloptUnif]
	{
	\Phi = 
	e^{-\epsilon(1 - 11B\eta)} \pi_2(\varu_2) \leq \pi_3 (\varu_1) 
		\land 
	e^{-\epsilon(1 - 11B\eta)} \pi_2 (\varu_1) \leq \pi_3 (\varu_2)
	}
	{
		\varu_1 \samplel \uniform(0,1)
		\sim_{\epsilon - 11B\eta\epsilon, 0} 
		\varu_2 \samplel \uniform(0,1)
		: 
		\top
		\Rightarrow 
		\Phi
	}
	~~
	\inferrule[FloptNull]
	{
	\empty
	}
	{
		s_1 = \samplel \uniform\{-1, 1\}
		\sim_{0, 0} 
		s_2 = \samplel \uniform\{-1, 1\}
		: 
		\Phi
		\Rightarrow 
		\Phi \land \pi_1(s_1) = \pi_1(s_2)
	}
	}
	{
		\varu_1 \samplel \uniform(0,1); s_1 = \samplel \uniform\{-1, 1\}
		\sim_{\epsilon - 11B\eta\epsilon, 0} 
		\varu_2 \samplel \uniform(0,1); s_2 = \samplel \uniform\{-1, 1\}
		: \top \Rightarrow \Phi \land \pi_1(s_1) = \pi_1(s_2)
	}
\\
\Pi_R
}
{
	\vdash 
	\varu_1 \samplel \uniform(0,1); s_1 = \samplel \uniform\{-1, 1\};
	\varx_1 = \clamp_B \big(
	\round{f(a) + \frac{1}{\epsilon} \times s_1 \times \ln (\varu_1)}_{\Lambda}
	\big) 
	\sim_{\epsilon - 11B\eta\epsilon, 0} 
	\varu_2 \samplel \uniform(0,1); s_2 = \samplel \uniform\{-1, 1\};
	\varx_2 = \clamp_B \big(
	\round{f(a') + \frac{1}{\epsilon} \times s_2 \times \ln (\varu_2)}_{\Lambda}
	: \top  \Rightarrow  \pi_1(\varx_1) = \pi_1(\varx_2)
}
\\
\Pi_R:
\\
\inferrule*[right = ConSeq]
{	
\inferrule*[right = Assn]
	{
		\Phi' = 
		e^{-\epsilon(1 - 11B\eta)} 
		e^{\epsilon (\frac{\pi_1(\varx_2)}{(1 + \eta)^3} - \frac{f(a')}{(1 + \eta)^2})}
		\leq 
		e^{\pi_1(\varx_1)(1 + \eta)^3 - f(a)(1 + \eta)^2}
		\land 
		e^{\epsilon(1 - 11B\eta)} 
		e^{\epsilon (\frac{\pi_1(\varx_1)}{(1 + \eta)^3} - \frac{f(a)}{(1 + \eta)^2})}
		\leq 
		e^{\pi_1(\varx_2)(1 + \eta)^3 - f(a')(1 + \eta)^2}
	}
	{
		\pi_1(\varx_1) = \clamp_B \big(
		\round{f(a) + \frac{1}{\epsilon} \times s_1 \times \ln (\varu_1)}_{\Lambda}
		\big) 
		\sim_{0, 0} 
		\pi_1(\varx_2) = \clamp_B \big(
		\round{f(a') + \frac{1}{\epsilon} \times s_2 \times \ln (\varu_2)}_{\Lambda}
		:
		\Phi \land \pi_1(s_1) = \pi_1(s_2)
		\Rightarrow
		\Phi'
	}
\and
\mathtodo{ \Phi' \Rightarrow \pi_1(\varx_1) = \pi_1(\varx_2)}
\\
\Phi \land \pi_1(s_1) = \pi_1(s_2)
\Rightarrow \Phi \land \pi_1(s_1) = \pi_1(s_2)
}
{
	\varx_1 = \clamp_B \big(
	\round{f(a) + \frac{1}{\epsilon} \times s_1 \times \ln (\varu_1)}_{\Lambda}
	\big) 
	\sim_{0, 0} 
	\varx_2 = \clamp_B \big(
	\round{f(a') + \frac{1}{\epsilon} \times s_2 \times \ln (\varu_2)}_{\Lambda}
	:
	\Phi \land \pi_1(s_1) = \pi_1(s_2)
	\Rightarrow \pi_1(\varx_1) = \pi_1(\varx_2)
}
\end{mathpar}
}
\todo{
	given that:
	$
	\Phi = 
	e^{-\epsilon(1 + 24B\eta)} \pi_2(\varu_2) \leq \pi_3 (\varu_1) 
		\land 
	e^{-\epsilon(1 + 24B\eta)} \pi_2 (\varu_1) \leq \pi_3 (\varu_2)
	$
	I'm only able to prove that:
	$\varx_1 = \varx_2 \Rightarrow \Phi'$
	but not 
	$\Phi' \Rightarrow \varx_1 = \varx_2$.
	\\
	However, given
	$ 
	\Phi = 
	e^{-\epsilon(1 - 11B\eta)} \pi_2(\varu_2) \leq \pi_3 (\varu_1) 
		\land 
	e^{-\epsilon(1 - 11B\eta)} \pi_2 (\varu_1) \leq \pi_3 (\varu_2)
	$, we are able to prove:
	$\Phi \implies \Phi' \implies \varx_1 = \varx_2$.
}
\\
Proof of \todo{ $\Phi' \Rightarrow \varx_1 = \varx_2$}:
\\
By the semantics definition of $\varu \samplel \uniform(0,1)$ and $\varx = \expr$, we have
the semantics of the pair of the snap programs as (given the input environment as empty):
\\
\[
\begin{array}{ll}
	& \sem{\varu_1 \samplel \uniform(0,1); s_1 = \samplel \uniform\{-1, 1\};
		\varx_1 = \clamp_B \big(
		\round{f(a) + \frac{1}{\epsilon} \times s_1 \times \ln (\varu_1)}_{\Lambda}
		\big)}_{[]} =
	\\
	&
	 \elet (\fval_1, \rval_1, \rval_1 ) = \sem{\uniform(0,1)}_{[]} 
	 \ein \elet (1, 1, 1) = \sem{\uniform\{-1, 1\}} \ein
	 [\varu_1 \mapsto (\fval_1, \rval_1, \rval_1); 
	 s_1 \mapsto (1, 1, 1); 
	 \varx_1 \mapsto \bigg(
				f(a) + \frac{1}{\epsilon} \times \ln(\fval_1),
				%
				 (f(a) + 
				(\frac{1}{\epsilon} \times \ln(\rval_1))
				(1 + \eta)^2)
				{(1 + \eta)},
				%
				\frac{(
				f(a) + \frac{\frac{1}{\epsilon} 
				\times \ln(\rval_1)}
				{(1 + \eta)^2}
				)}
				{(1 + \eta)}
				\bigg)]
	\\
	\sim
	&
	\sem{\varu_2 \samplel \uniform(0,1); s_2 = \samplel \uniform\{-1, 1\};
		\varx_2 = \clamp_B \big(
		\round{f(a') + \frac{1}{\epsilon} \times s_2 \times \ln (\varu_2)}_{\Lambda}}
	\\
	&
	\elet (\fval_2, \rval_2, \rval_2) = \sem{\uniform(0,1)}_{[]}
	\ein \elet (1, 1, 1) = \sem{\uniform\{-1, 1\}} \ein
	[\varu_2 \mapsto (\fval_2, \rval_2, \rval_2);
	 s_2 \mapsto (1, 1, 1); 
	 \varx_2 \mapsto \bigg(
				f(a) + \frac{1}{\epsilon} \times \ln(\fval_2),
						%
				\big( (f(a') + 
				(\frac{1}{\epsilon} \times \ln(\rval_2))
				(1 + \eta)^2)
				{(1 + \eta)},
				%
				\frac{(
				f(a') + \frac{\frac{1}{\epsilon} 
				\times \ln(\rval_2)}
				{(1 + \eta)^2}
				)}
				{(1 + \eta)}
				 \big)
				\bigg)]	
	\end{array}
\]
We consider the first case of $\sem{\uniform\{-1, 1\}}_{[]} = (1, 1, 1)$ with probability 0.5.
\\
By the condition $\Phi$, we have:
\[
	e^{-\epsilon(1 - 11B\eta)} \pi_2(\varu_2) \leq \pi_3 (\varu_1) 
	\land 
	e^{-\epsilon(1 - 11B\eta)} \pi_2 (\varu_1) \leq \pi_3 (\varu_2)
\]
i.e.,
\[
	e^{-\epsilon(1 - 11B\eta)} \rval_2 \leq \rval_1
	\leq e^{\epsilon(1 - 11B\eta)} \rval_2
	 ~ (\star)
\]
By the soundness of the transition semantics, we have:
\[
	(f(a) + (\frac{1}{\epsilon} \times \ln(\rval_1))
	(1 + \eta)^2){(1 + \eta)}
	\leq \varx_1 \leq
	\frac{(f(a) + \frac{\frac{1}{\epsilon} 
	\times \ln(\rval_1)}{(1 + \eta)^2})}
	{(1 + \eta)}
	~~ \sim ~~
	(f(a') + (\frac{1}{\epsilon} \times \ln(\rval_2))
	(1 + \eta)^2){(1 + \eta)}
	\leq \varx_2 \leq
	\frac{(f(a') + \frac{\frac{1}{\epsilon} 
	\times \ln(\rval_2)}
	{(1 + \eta)^2} )}{(1 + \eta)}
\]
Then, we can get:
\[
	e^{\epsilon(\varx_1 (1 + \eta)^3 - f(a)(1 + \eta)^2)}
	\leq \rval_1 \leq
	e^{\epsilon(\frac{\varx_1}{(1 + \eta)^3}  - \frac{f(a)}{(1 + \eta)^2})}
	~~ \sim ~~
	e^{\epsilon(\varx_2 (1 + \eta)^3 - f(a')(1 + \eta)^2)}
	\leq \rval_2 \leq
	e^{\epsilon(\frac{\varx_2}{(1 + \eta)^3}  - \frac{f(a')}{(1 + \eta)^2})} ~ (\diamond)
\]
According to $(\star)$ and $(\diamond)$, we have:
\[
		e^{-\epsilon(1 - 1B\eta)} 
		e^{\epsilon (\frac{\varx_2}{(1 + \eta)^3} - \frac{f(a')}{(1 + \eta)^2})}
		\leq 
		e^{\varx_1(1 + \eta)^3 - f(a)(1 + \eta)^2}
		~~ \land ~~
		e^{\epsilon(1 - 11B\eta)} 
		e^{\epsilon (\frac{\varx_1}{(1 + \eta)^3} - \frac{f(a)}{(1 + \eta)^2})}
		\leq 
		e^{\varx_2(1 + \eta)^3 - f(a')(1 + \eta)^2} ~ (\Phi')
\]
By simplifying, we have:
\[
	(\Phi')	
	~~ \implies ~~
	\varx_2 \leq \varx_1 \leq \varx_2 
	~~ \implies ~~
	\varx_2 = \varx_1
\]

\end{proof}

\newpage
\bibliographystyle{plain}
\bibliography{verifysnap.bib}

\end{document}



